dimsum/universes.v
@@ -1,0 +1,20 @@
+From iris.algebra Require Import ofe.
+From dimsum Require Import base.
+
+Module Import universes.
+  (** The universe of the state of modules. *)
+  Universe State.
+  (** The universe of events. *)
+  Universe Event.
+  (** The universe of ordinals. *)
+  Universe Ordinal.
+End universes.
+
+Notation TypeState := Type@{State} (only parsing).
+Notation TypeEvent := Type@{Event} (only parsing).
+Notation TypeOrdinal := Type@{Ordinal} (only parsing).
+Notation TypeOfe := Type@{ofe.u0} (only parsing).
+
+Constraint State < Ordinal.
+(* TODO: add this constraint here once itrees are compatible with it *)
+(* Constraint Ordinal <= ofe.u0. *)
